



Eq 1 from (1)

$$6 - 3I_1 + 0I_2 + 5I_3 + 0I_4 = 0$$

Eq 2 from (2)

$$-5I_3 - 4(I_1 + I_3) + 2(I_4 - I_2) = 0$$

$$\Rightarrow -4I_1 - 2I_2 - 9I_3 + 2I_4 = 0$$

Eq. 3 from (3)

$$-2(I_4 - I_2) - 1 \cdot I_4 - 3 = 0$$

$$\Rightarrow -3 + 0I_1 + 2I_2 + 0I_3 - 3I_4 = 0$$

Eq. 4 from 4:

$$I_1 + I_3 = I_2$$

$$\Rightarrow I_1 - I_2 + I_3 + 0I_4 = 0$$

$$\begin{bmatrix} -3 & 0 & 5 & 0 \\ -4 & -2 & -9 & 2 \\ 0 & 2 & 0 & -3 \\ 1 & -1 & 1 & 0 \end{bmatrix} \begin{bmatrix} I_1 \\ I_2 \\ I_3 \\ I_4 \end{bmatrix} = \begin{bmatrix} -6 \\ 0 \\ 3 \\ 0 \end{bmatrix}$$